lab-2-data-structures/BST_list_proof.v
@@ -1,0 +1,97 @@
+
+
+Require Import DataStructures.Int.
+Require Import DataStructures.Red_black_tree.
+Require Import DataStructures.Red_black_tree_proof.
+Import Red_black_tree.
+Require Import Coq.Logic.FunctionalExtensionality.
+Require Import Lia.
+Require Import List.
+Import ListNotations.
+Import Red_black_tree_proof.
+
+Module BST_list_proofs.
+
+Search (In _ (_ ++ _)).  
+
+Search app.
+
+Search ((_, _) = (_, _)).
+
+Search incl.
+
+Lemma elemets_complete {V: Type} (k: key) (v: V) (t: rbtree V) :
+  lookup k t = Some v -> In (k,v) (elements t).
+Proof.
+    unfold elements. 
+    generalize dependent k.
+    generalize dependent v.
+    induction t as [| c l IHl k0 v0 r IHr]; simpl.
+    - intros. discriminate.
+    - intros v k. destruct (ltb k k0) eqn: Hlt.
+      all: destruct (ltb k0 k) eqn: Hgt.
+      +  apply ltb_lt in Hlt, Hgt; lia.
+      +  clear IHr.
+         intros Hlookup.
+         apply IHl in Hlookup.
+         apply in_or_app.
+         left; auto.
+      + clear IHl.
+        intros Hlookup.
+        apply IHr in Hlookup.
+        apply in_or_app; auto.
+        right.
+        apply in_cons; auto.
+      + apply ltb_f_lt in Hlt, Hgt; auto.
+        intros Hveq.
+        assert(Heq: (k, v) = (k0, v0)).
+        ++ apply pair_equal_spec. split.
+        +++ assert (Hkeq: (mk_z k0) = (mk_z k)). {apply BinInt.Z.le_antisymm; auto. }
+            apply mk_z_inj; auto.
+        +++ congruence. 
+        ++ rewrite Heq. apply in_elt; auto.
+Qed.
+
+Definition uncurry {X Y Z : Type} (f : X -> Y -> Z) '(a, b) :=
+  f a b.
+Hint Transparent uncurry : core.
+
+Search Forall.
+
+Lemma elements_forall {V : Type}: forall (P : key -> V -> Prop) (t : rbtree V),
+    ForallT P t ->
+    Forall (uncurry P) (elements t).
+Proof.
+  intros P t.
+  unfold elements.
+  induction t as [| c l IHl k v r IHr]; auto.
+  intros HForall.
+  inversion HForall. clear HForall. subst.
+  destruct H0 as [Hl Hr].
+  apply IHl in Hl.
+  apply IHr in Hr.
+  apply Forall_app. split; auto.
+  apply Forall_cons; auto.
+Qed.
+
+
+Lemma elements_relation {V : Type}: forall   (R : key -> key -> Prop) 
+      (v: V) (t : rbtree V) 
+      (k' k: key) ,
+    ForallT (fun y _ => R y k') t ->
+    In (k, v) (elements t) -> R k k'.
+Proof.
+  intros R v t k' k.
+  
+     
+
+
+
+Lemma elemets_correct {V: Type}:
+  forall (k: key) (v: V) (t: rbtree V),
+  BST t -> In (k, v) (elements t) -> lookup k t = Some v.
+Admitted.
+    
+
+
+End BST_list_proofs.
